

Serie N°3 Numerical Series

Ex 1:

$$① U_n = \frac{\cos \alpha n}{2^n}, \quad \alpha \in \mathbb{R}$$

$$= \operatorname{Re} \left[\left(\frac{1}{2} e^{i\alpha} \right)^n \right]$$

$$V_n = \sum_{k=0}^n U_k = \sum_{k=0}^n \operatorname{Re} (q^k) / q = \frac{1}{2} e^{i\alpha}$$

$$= \operatorname{Re} \left(\sum_{k=0}^n q^k \right) = \operatorname{Re} \left(\frac{q^{n+1} - 1}{q - 1} \right) \quad \text{because } |q| = \frac{1}{2}$$

$$= \operatorname{Re} \left(\frac{1 - q^{n+1}}{1 - q} \right)$$

$$\lim V_n = \operatorname{Re} \left(\frac{1}{1 - q} \right) \quad \text{because } |q^{n+1}| = \frac{1}{2^{n+1}}$$

$$\sum_{n=0}^{+\infty} \frac{\cos n\alpha}{2^n} = \operatorname{Re} \left(\frac{1}{1 - \frac{1}{2} \cos \alpha - i \frac{1}{2} \sin \alpha} \right)$$

$$= \frac{1 - \frac{1}{2} \cos \alpha}{(1 - \frac{1}{2} \cos \alpha)^2 + (\frac{1}{2} \sin \alpha)^2}$$

$$\sum_{n=0}^{+\infty} \frac{\cos n\alpha}{2^n} = \frac{1 - \frac{1}{2} \cos \alpha}{1 + \frac{1}{4} - \cos \alpha}$$

$$= \frac{\frac{1}{2} (2 - \cos \alpha)}{\frac{5}{4} - \cos \alpha}$$

$$\sum_{n=0}^{+\infty} \frac{\cos n\alpha}{2^n} = \frac{4 - 2 \cos \alpha}{5 - 4 \cos \alpha}$$

$$\operatorname{Re} \left(\frac{1}{z} \right) = \operatorname{Re} \left(\frac{\bar{z}}{|z|^2} \right)$$

$$= \frac{1}{|z|^2} \operatorname{Re} (\bar{z})$$

$$= \frac{\operatorname{Re} (\bar{z})}{|z|^2}$$

$$u_n = (1+n)q^n$$

$$(2) \quad u_n = \frac{n+1}{3^n}$$

$$\sum_{n=0}^{+\infty} u_n = \left(\frac{1}{1-q} \right)^2 = \frac{1}{(1-q)^2}$$

$$q = \frac{1}{3} \quad \sum_{n=0}^{+\infty} \frac{n+1}{3^n} = \frac{1}{(1-\frac{1}{3})^2} = \frac{9}{4}$$

$$\frac{1}{(1-q)^2} = \left(\sum_{n=0}^{+\infty} q^n \right)^2 = \sum_{n=0}^{+\infty} q^n \times q^n$$

$$= \sum_{n=0}^{+\infty} \left[\sum_{k=0}^n q^k \cdot q^{n-k} \right]$$

$$= \sum_{n=0}^{+\infty} q^n (1 + \underbrace{1 + \dots + 1}_{n+1}) = \sum_{n=0}^{+\infty} (n+1)q^n$$

$$(3) \quad u_n = \frac{n - (-1)^n}{3^n} = \frac{n+1}{3^n} - \frac{1+(-1)^n}{3^n}$$

$$\sum_{n=0}^{+\infty} u_n = \sum_{n=0}^{+\infty} \frac{n+1}{3^n} - \sum_{n=0}^{+\infty} \frac{1+(-1)^n}{3^n}$$

$$= \frac{9}{4} - \sum_{n=0}^{+\infty} \frac{2}{3^{2n}} = \frac{9}{4} - 2 \sum_{n=0}^{+\infty} \frac{1}{9^n}$$

$$= \frac{9}{4} - 2 \left(\frac{1}{1-\frac{1}{9}} \right) = \frac{9}{4} - 2 \times \frac{9}{8} = \frac{1}{4}$$

$$(4) \quad u_n = \frac{n}{n^4 + n^2 + 1} = \frac{n}{(n^2 + n + 1)(n^2 - n + 1)}$$

$$= \frac{n}{(n^2 + 1)^2 - n^2} = \frac{n}{(n^2 - n + 1)(n^2 + n + 1)}$$

$$= \frac{1}{2} \times \frac{(n^2 + n + 1) - (n^2 - n + 1)}{(n^2 - n + 1)(n^2 + n + 1)}$$

$$= \frac{1}{2} \left[\frac{1}{n^2 - n + 1} - \frac{1}{n^2 + n + 1} \right]$$

$$= a_n - a_{n+1} \quad a_n = \frac{1}{2} \times \frac{1}{n^2 - n + 1} = \frac{1}{2(n+1)(n-1)}$$

$$a_{n+1} = \frac{1}{2(1+n(n+1))}$$

$$u_n = (a_0 - a_1) + (a_1 - a_2) + \dots + (a_{n-1} - a_n) + (a_n - a_{n+1})$$

$$u_n = a_0 - a_{n+1} = \frac{1}{2} - \frac{1}{2(1+n(n+1))}$$

$$\lim_{n \rightarrow \infty} u_n = \frac{1}{2} = \sum_{n=0}^{+\infty} \frac{n}{n^4 + n^2 + 1}$$

$$(5) \quad \sum_{k=1}^n k^3 = \left(\sum_{k=1}^n k \right)^2$$

$$u_n = \frac{\sum_{k=1}^n k}{\left(\sum_{k=1}^n k \right)^2} = \frac{1}{\sum_{k=1}^n k}$$

$$= \frac{1}{\frac{n(n+1)}{2}} = \frac{2}{n(n+1)} = 2 \left(\frac{1}{n} - \frac{1}{n+1} \right)$$

$$= a_n - a_{n+1}$$

$$\sum_{n=1}^{+\infty} u_n = a_1 - \lim_{n \rightarrow \infty} a_{n+1} = 2 - 0 = 2$$

$$(6) \quad u_n = \ln(1 - n^{-2}) = \ln\left(1 - \frac{1}{n^2}\right)$$

$$= \ln\left(1 - \frac{1}{n}\right) + \ln\left(1 + \frac{1}{n}\right)$$

$$= \ln\left(\frac{n-1}{n}\right) + \ln\left(\frac{n+1}{n}\right)$$

$$= \ln\left(\frac{n-1}{n}\right) - \ln\left(\frac{n}{n+1}\right) = a_n - a_{n+1}$$

$$u_n = a_n - a_{n+1} = a_2 - \ln\left(\frac{n}{n+1}\right)$$

$$a_2 = \ln \frac{1}{2} = -\ln 2$$

$$(7) \quad u_n = \ln n + a \ln(n+2) + b \ln(n+3)$$

$$\sum u_n \text{ Cr} \Rightarrow \lim_{n \rightarrow \infty} u_n = 0$$

$$u_n = \ln n + a \left[\ln n + \ln\left(1 + \frac{2}{n}\right) \right]$$

$$+ b \left[\ln n + \ln\left(1 + \frac{3}{n}\right) \right]$$

$$= (1+a+b) \ln n + a \ln\left(1 + \frac{2}{n}\right) + b \ln\left(1 + \frac{3}{n}\right)$$

$$1+a+b=0 \quad \begin{cases} 1+a+b \neq 0 \\ \infty \\ a \\ b \end{cases}$$

$$u_n = (1+n)q^n$$

$$(2) \quad u_n = \frac{n+1}{3^n}$$

$$\sum_{n=0}^{\infty} u_n = \left(\frac{1}{1-q} \right)^2 = \frac{1}{(1-q)^2}$$

$$q = \frac{1}{3} \quad \sum_{n=0}^{\infty} \frac{n+1}{3^n} = \frac{1}{(1-\frac{1}{3})^2} = \frac{9}{4}$$

$$\frac{1}{(1-q)^2} = \left(\sum_{n=0}^{\infty} q^n \right)^2 = \sum_{n=0}^{\infty} q^n \times q^n$$

$$= \sum_{n=0}^{\infty} \left[\sum_{k=0}^n q^k \cdot q^{n-k} \right]$$

$$= \sum_{n=0}^{\infty} q^n (1 + \dots + 1) = \sum_{n=0}^{\infty} (n+1)q^n$$

$$(3) \quad u_n = \frac{n - (-1)^n}{3^n} = \frac{n+1}{3^n} - \frac{1+(-1)^n}{3^n}$$

$$\sum_{n=0}^{\infty} u_n = \sum_{n=0}^{\infty} \frac{n+1}{3^n} - \sum_{n=0}^{\infty} \frac{1+(-1)^n}{3^n}$$

$$= \frac{9}{4} - \sum_{n=0}^{\infty} \frac{2}{3^n} = \frac{9}{4} - 2 \sum_{n=0}^{\infty} \frac{1}{3^n}$$

$$= \frac{9}{4} - 2 \left(\frac{1}{1-\frac{1}{3}} \right) = \frac{9}{4} - 2 \times \frac{3}{2} = \frac{9}{4} - 3 = \frac{9}{4} - \frac{12}{4} = -\frac{3}{4}$$

$$(4) \quad u_n = \frac{n}{n^4 + n^2 + 1} = \frac{n}{(n^2 + n + 1)(n^2 - n + 1)}$$

$$= \frac{n}{(n^2 + 1)^2 - n^2} = \frac{n}{(n^2 - n + 1)(n^2 + n + 1)}$$

$$= \frac{1}{2} \times \frac{(n^2 + n + 1) - (n^2 - n + 1)}{(n^2 - n + 1)(n^2 + n + 1)}$$

$$= \frac{1}{2} \left[\frac{1}{n^2 - n + 1} - \frac{1}{n^2 + n + 1} \right]$$

$$= a_n - a_{n+1} \quad a_n = \frac{1}{2} \times \frac{1}{n^2 - n + 1} = \frac{1}{2(n-1)(n+1)}$$

$$a_{n+1} = \frac{1}{2(1+n(n+1))}$$

$$u_n = (a_0 - a_1) + (a_1 - a_2) + \dots + (a_n - a_{n+1})$$

$$u_n = a_0 - a_{n+1} = \frac{1}{2} - \frac{1}{2(1+n(n+1))}$$

$$\lim_{n \rightarrow \infty} u_n = \frac{1}{2} = \sum_{n=0}^{\infty} \frac{n}{n^4 + n^2 + 1}$$

$$(5) \quad \sum_{k=1}^n k^3 = \left(\sum_{k=1}^n k \right)^2$$

$$u_n = \frac{\sum_{k=1}^n k}{\left(\sum_{k=1}^n k \right)^2} = \frac{1}{\sum_{k=1}^n k}$$

$$= \frac{1}{\frac{n(n+1)}{2}} = \frac{2}{n(n+1)} = 2 \left(\frac{1}{n} - \frac{1}{n+1} \right)$$

$$= a_n - a_{n+1}$$

$$\sum_{n=1}^{\infty} u_n = a_1 - \lim_{n \rightarrow \infty} a_{n+1} = 2 - 0 = 2$$

$$(6) \quad u_n = \ln(1 - n^{-2}) = \ln\left(1 - \frac{1}{n^2}\right)$$

$$= \ln\left(1 - \frac{1}{n}\right) + \ln\left(1 + \frac{1}{n}\right)$$

$$= \ln\left(\frac{n-1}{n}\right) + \ln\left(\frac{n+1}{n}\right)$$

$$= \ln\left(\frac{n-1}{n}\right) - \ln\left(\frac{n}{n+1}\right) = a_n - a_{n+1}$$

$$u_n = a_n - a_{n+1} = a_2 - \ln\left(\frac{n}{n+1}\right)$$

$$a_2 = \ln \frac{1}{2} = -\ln 2$$

$$(7) \quad u_n = \ln n + a \ln(n+2) + b \ln(n+3)$$

$$\sum u_n \text{ Cr} \Rightarrow \lim_{n \rightarrow \infty} u_n = 0$$

$$u_n = \ln n + a \left[\ln n + \ln\left(1 + \frac{2}{n}\right) \right]$$

$$+ b \left[\ln n + \ln\left(1 + \frac{3}{n}\right) \right]$$

$$= (1+a+b) \ln n + a \ln\left(1 + \frac{2}{n}\right) + b \ln\left(1 + \frac{3}{n}\right)$$

$$1+a+b=0$$

$$1+a+b \neq 0$$

$$a$$

$$b$$

$$\sum u_n \text{ cv} \Rightarrow a+b+1=0$$

$$\Rightarrow b = -1-a$$

$$\text{So when } b = -1-a$$

$$\begin{aligned} u_n &= \ln n + a \ln(n+2) - (a+1) \ln(n+3) \\ &= \ln n + a \ln(n+2) - \ln(n+3) - a \ln(n+3) \\ &= \ln n - \ln(n+3) + a [\ln(n+2) - \ln(n+3)] \\ &= \ln n - \ln(n+3) + \ln(n+1) - \ln(n+2) + \ln(n+2) \\ &\quad - \ln(n+3) + a \ln(n+2) - a \ln(n+3) \end{aligned}$$

$$\begin{aligned} &= [\ln n + \ln(n+1) + (a+1) \ln(n+2)] \\ &\quad - [\ln(n+1) + \ln(n+2) + (a+1) \ln(n+3)] \\ &= a_n - a_{n+1} = a_n - a_{n+1}, \forall n \geq 1 \end{aligned}$$

$$u_n = a_n - a_{n+1} = a_n - a_{n+1}$$

$$\sum u_n \text{ cv} \Leftrightarrow (a_n)_{n \in \mathbb{N}} \text{ cv}$$

$$\begin{aligned} a_{n+1} &= \ln(n+1) + \ln(n+2) + (a+1) \ln(n+3) \\ &= (a+3) \ln n + [\ln(1+\frac{1}{n}) + \ln(1+\frac{2}{n}) \\ &\quad + (a+1) \ln(1+\frac{3}{n})] \end{aligned}$$

$$\sum u_n \text{ cv} \Rightarrow a+3=0 \Rightarrow a=-3$$

$$b=2$$

$$\sum_{n=1}^{\infty} u_n = \ln 2 - 2 \ln 3 = \ln \frac{2}{9}$$

Ex 2:

$$\begin{aligned} \text{1) } u_n &= \sqrt{n^2+n} - n = \frac{n}{\sqrt{n^2+n} + n} \\ &= \frac{1}{1 + \sqrt{1 + \frac{1}{n}}} \end{aligned}$$

$$\lim u_n = \frac{1}{2} \neq 0 \Rightarrow \sum u_n \text{ div}$$

$$\text{2) } u_n = \frac{\ln n}{n^2} \quad (\text{The Bertrand series})$$

$$u_n = \frac{1}{n^{\alpha}} \times \frac{\ln n}{n^{\beta}} = o\left(\frac{1}{n^{\alpha+\beta}}\right)$$

$$\sum_{n \in \mathbb{N}} \frac{1}{n^{\alpha+\beta}} = \sum_{n \in \mathbb{N}} \frac{1}{n^{\alpha+\beta}} \quad (\text{The Riemann series})$$

$$\sum u_n \text{ cv}$$

$$\text{3) } u_n = \frac{1 + \ln n}{\sqrt{n}} \gg \frac{1}{\sqrt{n}} = \frac{1}{n^{1/2}}$$

$$\frac{1}{2} < 1 \Rightarrow \sum \frac{1}{\sqrt{n}} \text{ div} \Rightarrow \sum u_n \text{ div}$$

(comparison criterion)

$$\begin{aligned} \text{4) } u_n &= \frac{n + \sqrt{n}}{2n^3 - 1} = \frac{n(1 + \frac{1}{\sqrt{n}})}{2n^3(1 - \frac{1}{2n^3})} \\ &= \frac{1}{2n^2} \times \frac{1 + \frac{1}{\sqrt{n}}}{1 - \frac{1}{2n^3}} \sim \frac{1}{2n^2} \end{aligned}$$

$$\sum \frac{1}{2n^2} \text{ cv} \Rightarrow \sum u_n \text{ cv}$$

(equivalence criterion)

$$\begin{aligned} \text{5) } u_n &= (\sqrt{2} + \sqrt{3})^{-n^2} \\ \rightarrow \sqrt[n]{u_n} &= (\sqrt{3} + \sqrt{2})^{-n} \end{aligned}$$

$$\begin{aligned} &= \frac{1}{(\sqrt{3} + \sqrt{2})^n} = \frac{1}{[\sqrt{3}(1 + \sqrt{\frac{2}{3}})]^n} \\ &= \frac{1}{3(1 + \sqrt{\frac{2}{3}})^n} \end{aligned}$$

by Cauchy's criterion

$$\sum u_n \text{ cv}$$

$$\text{6) } u_n = \frac{(n+1)(n+2)}{(2n)^n} = \frac{(2n+2)}{(2n)^n}$$

$$\frac{u_{n+1}}{u_n} = \frac{(n+2)(n+3)}{(2n+2)^{n+1}} \cdot \frac{(2n)^n}{(2n+2)}$$

$$= \frac{[(n+2)(n+3) - (2n)(2n+1)(2n+2)] (e n)^n}{(n+1)(n+2) \dots (2n) (2n+2)^n (2n+2)}$$

$$= \frac{2n+1}{n+1} \times \frac{(2n)^n}{(2n+2)^n} = \frac{2n+1}{n+1} \times \frac{1}{\left(1+\frac{1}{n}\right)^n}$$

$$\rightarrow \frac{2}{e} < 1$$

So $\sum u_n$ Cv